src/Step.hs
@@ -1,39 +1,6 @@
-{-# OPTIONS_GHC -cpp -XMagicHash #-}
-{- For Hugs, use the option -F"cpp -P -traditional" -}
-
 module Step where
 
 import qualified Prelude
-
-#ifdef __GLASGOW_HASKELL__
-import qualified GHC.Base
-#else
--- HUGS
-import qualified IOExts
-#endif
-
-#ifdef __GLASGOW_HASKELL__
-unsafeCoerce :: a -> b
-unsafeCoerce = GHC.Base.unsafeCoerce#
-#else
--- HUGS
-unsafeCoerce :: a -> b
-unsafeCoerce = IOExts.unsafeCoerce
-#endif
-
-#ifdef __GLASGOW_HASKELL__
-type Any = GHC.Base.Any
-#else
--- HUGS
-type Any = ()
-#endif
-
-__ :: any
-__ = Prelude.error "Logical or arity value used"
-
-eq_rect :: a1 -> a2 -> a1 -> a2
-eq_rect _ f _ =
-  f
 
 type EqDec v =
   v -> v -> Prelude.Bool
@@ -43,217 +10,47 @@ eq_decide :: (EqDec a1) -> a1 -> a1 -> Prelude.Bool
 eq_decide eqDec =
   eqDec
 
-type Functor f =
-  () -> () -> (Any -> Any) -> f -> f
-  -- singleton inductive, whose constructor was Build_Functor
-  
-map :: (Functor a1) -> (a2 -> a3) -> a1 -> a1
-map functor x x0 =
-  unsafeCoerce functor __ __ x x0
-
-data Monad m =
-   Build_Monad (() -> Any -> m) (() -> m -> m)
-
-pure :: (Functor a1) -> (Monad a1) -> a2 -> a1
-pure _ monad x =
-  case monad of {
-   Build_Monad pure0 _ -> unsafeCoerce pure0 __ x}
-
-join :: (Functor a1) -> (Monad a1) -> a1 -> a1
-join _ monad x =
-  case monad of {
-   Build_Monad _ join0 -> join0 __ x}
-
-type State s a = s -> (,) s a
-
-get :: State a1 a1
-get x =
-  (,) x x
-
-put :: a1 -> State a1 ()
-put x _ =
-  (,) x ()
-
-state_Functor :: Functor (State a1 Any)
-state_Functor _ _ f x s0 =
-  case x s0 of {
-   (,) s1 y -> (,) s1 (f y)}
-
-state_Monad :: Monad (State a1 Any)
-state_Monad =
-  Build_Monad (\_ x s0 -> (,) s0 x) (\_ a s0 ->
-    case a s0 of {
-     (,) s1 b -> unsafeCoerce b s1})
-
 data Term v =
    Var v
  | App (Term v) (Term v)
- | Lam v (Term v)
+ | Lam_ (v -> Term v)
 
-data D v =
-   Var'
- | Lapp' (Term v) (Term v) (D v)
- | Rapp' (Term v) (Term v) (D v)
- | Lam' v (Term v) (D v)
+type Store v = v -> Term v
 
-diff :: a1 -> (Term a1) -> (Term a1) -> (D a1) -> Term a1
-diff x h _ i =
-  case i of {
-   Var' -> h;
-   Lapp' e0 e1 i0 -> App (diff x h e0 i0) e1;
-   Rapp' e0 e1 i1 -> App e0 (diff x h e1 i1);
-   Lam' y e0 i0 -> Lam y (diff x h e0 i0)}
+data Font v =
+   Build_font v (Font v) (Font v)
 
-var_helper :: a1 -> a1 -> D a1
-var_helper x y =
-  eq_rect x Var' y
+head :: (Font a1) -> a1
+head f =
+  case f of {
+   Build_font head0 _ _ -> head0}
 
-lookup :: a1 -> (EqDec a1) -> (Term a1) -> Prelude.Maybe (D a1)
-lookup x h e =
+left :: (Font a1) -> Font a1
+left f =
+  case f of {
+   Build_font _ left0 _ -> left0}
+
+insert :: (EqDec a1) -> a1 -> (Term a1) -> (a1 -> Term a1) -> Store a1
+insert h x e s x' =
+  case eq_decide h x x' of {
+   Prelude.True -> e;
+   Prelude.False -> s x'}
+
+cbn :: (EqDec a1) -> (Font a1) -> (Term a1) -> (Store a1) -> Prelude.Maybe
+       ((,) (Store a1) (Term a1))
+cbn h xs e s0 =
   case e of {
-   Var y ->
-    case eq_decide h x y of {
-     Prelude.True -> Prelude.Just (var_helper x y);
-     Prelude.False -> Prelude.Nothing};
-   App e0 e1 ->
-    let {s = lookup x h e0} in
-    let {s0 = lookup x h e1} in
-    case s of {
-     Prelude.Just e'0 -> Prelude.Just (Lapp' e0 e1 e'0);
-     Prelude.Nothing ->
-      case s0 of {
-       Prelude.Just e'1 -> Prelude.Just (Rapp' e0 e1 e'1);
-       Prelude.Nothing -> Prelude.Nothing}};
-   Lam y e0 ->
-    case lookup x h e0 of {
-     Prelude.Just e'0 -> Prelude.Just (Lam' y e0 e'0);
-     Prelude.Nothing -> Prelude.Nothing}}
-
-data Stream v =
-   Build_stream v (Stream v)
-
-head :: (Stream a1) -> a1
-head s =
-  case s of {
-   Build_stream head0 _ -> head0}
-
-tail :: (Stream a1) -> Stream a1
-tail s =
-  case s of {
-   Build_stream _ tail0 -> tail0}
-
-type Vars v a = State (Stream v) a
-
-vars_Functor :: Functor (Vars a1 Any)
-vars_Functor =
-  state_Functor
-
-vars_Monad :: Monad (Vars a1 Any)
-vars_Monad =
-  state_Monad
-
-alloc :: Vars a1 a1
-alloc =
-  join (unsafeCoerce vars_Functor) (unsafeCoerce vars_Monad)
-    (map (unsafeCoerce vars_Functor) (\s ->
-      join (unsafeCoerce vars_Functor) (unsafeCoerce vars_Monad)
-        (map (unsafeCoerce vars_Functor) (\_ ->
-          pure vars_Functor vars_Monad (head s)) (put (tail s))))
-      (unsafeCoerce get))
-
-free :: a1 -> Vars a1 ()
-free x =
-  join (unsafeCoerce vars_Functor) (unsafeCoerce vars_Monad)
-    (map (unsafeCoerce vars_Functor) (\s ->
-      join (unsafeCoerce vars_Functor) (unsafeCoerce vars_Monad)
-        (map (unsafeCoerce vars_Functor) (\_ ->
-          pure vars_Functor vars_Monad ()) (put (Build_stream x s))))
-      (unsafeCoerce get))
-
-replace :: a1 -> (EqDec a1) -> ([] ((,) a1 a1)) -> a1
-replace x h xs =
-  case xs of {
-   [] -> x;
-   (:) p t ->
-    case p of {
-     (,) y subst ->
-      case eq_decide h x y of {
-       Prelude.True -> subst;
-       Prelude.False -> replace x h t}}}
-
-rename :: (EqDec a1) -> ([] ((,) a1 a1)) -> (Term a1) -> Vars a1 (Term a1)
-rename h xs e =
-  case e of {
-   Var x ->
-    pure (unsafeCoerce vars_Functor) (unsafeCoerce vars_Monad) (Var
-      (replace x h xs));
-   App f x ->
-    join (unsafeCoerce vars_Functor) (unsafeCoerce vars_Monad)
-      (map (unsafeCoerce vars_Functor) (\f' ->
-        join (unsafeCoerce vars_Functor) (unsafeCoerce vars_Monad)
-          (map (unsafeCoerce vars_Functor) (\x' ->
-            pure vars_Functor vars_Monad (App f' x')) (rename h xs x)))
-        (rename h xs f));
-   Lam x e0 ->
-    join (unsafeCoerce vars_Functor) (unsafeCoerce vars_Monad)
-      (map (unsafeCoerce vars_Functor) (\x' ->
-        join (unsafeCoerce vars_Functor) (unsafeCoerce vars_Monad)
-          (map (unsafeCoerce vars_Functor) (\e' ->
-            pure vars_Functor vars_Monad (Lam x' e'))
-            (rename h ((:) ((,) x x') xs) e0))) (unsafeCoerce alloc))}
-
-destroy_term :: (Term a1) -> Vars a1 ()
-destroy_term e =
-  case e of {
-   Var _ -> pure (unsafeCoerce vars_Functor) (unsafeCoerce vars_Monad) ();
-   App e0 e1 ->
-    join (unsafeCoerce vars_Functor) (unsafeCoerce vars_Monad)
-      (map (unsafeCoerce vars_Functor) (\_ -> destroy_term e1)
-        (destroy_term e0));
-   Lam x e0 ->
-    join (unsafeCoerce vars_Functor) (unsafeCoerce vars_Monad)
-      (map (unsafeCoerce vars_Functor) (\_ -> free x) (destroy_term e0))}
-
-step :: (EqDec a1) -> (Term a1) -> Vars a1 (Prelude.Maybe (Term a1))
-step h e =
-  case e of {
-   Var _ ->
-    pure (unsafeCoerce vars_Functor) (unsafeCoerce vars_Monad)
-      Prelude.Nothing;
+   Var x -> Prelude.Just ((,) s0 (s0 x));
    App e0 e1 ->
     case e0 of {
-     Var _ ->
-      join (unsafeCoerce vars_Functor) (unsafeCoerce vars_Monad)
-        (map (unsafeCoerce vars_Functor) (\e'0 ->
-          pure vars_Functor vars_Monad
-            (case e'0 of {
-              Prelude.Just e''0 -> Prelude.Just (App e''0 e1);
-              Prelude.Nothing -> Prelude.Nothing})) (step h e0));
-     App _ _ ->
-      join (unsafeCoerce vars_Functor) (unsafeCoerce vars_Monad)
-        (map (unsafeCoerce vars_Functor) (\e'0 ->
-          pure vars_Functor vars_Monad
-            (case e'0 of {
-              Prelude.Just e''0 -> Prelude.Just (App e''0 e1);
-              Prelude.Nothing -> Prelude.Nothing})) (step h e0));
-     Lam x e2 ->
-      case lookup x h e2 of {
-       Prelude.Just ix ->
-        join (unsafeCoerce vars_Functor) (unsafeCoerce vars_Monad)
-          (map (unsafeCoerce vars_Functor) (\e'1 ->
-            join (unsafeCoerce vars_Functor) (unsafeCoerce vars_Monad)
-              (map (unsafeCoerce vars_Functor) (\e''1 ->
-                pure vars_Functor vars_Monad (Prelude.Just
-                  (let {e' = diff x e'1 e2 ix} in App (Lam x e') e''1)))
-                (rename h [] e1))) (unsafeCoerce rename h [] e1));
-       Prelude.Nothing ->
-        join (unsafeCoerce vars_Functor) (unsafeCoerce vars_Monad)
-          (map (unsafeCoerce vars_Functor) (\_ ->
-            join (unsafeCoerce vars_Functor) (unsafeCoerce vars_Monad)
-              (map (unsafeCoerce vars_Functor) (\_ ->
-                pure vars_Functor vars_Monad (Prelude.Just e2)) (free x)))
-            (unsafeCoerce destroy_term e1))}};
-   Lam _ _ ->
-    pure (unsafeCoerce vars_Functor) (unsafeCoerce vars_Monad)
-      Prelude.Nothing}
+     Lam_ f ->
+      let {v = head xs} in
+      let {y = f v} in Prelude.Just ((,) (insert h v e1 s0) y);
+     _ ->
+      case cbn h (left xs) e0 s0 of {
+       Prelude.Just p ->
+        case p of {
+         (,) s1 e'0 -> Prelude.Just ((,) s1 (App e'0 e1))};
+       Prelude.Nothing -> Prelude.Nothing}};
+   Lam_ _ -> Prelude.Nothing}
 
