lambda.v
@@ -142,9 +142,10 @@ Context { v : Set }.
 Inductive term : Set :=
 | var ( _ : v)
 | app (_ : term) (_ : term)
-| lam (_ : v) (_ : term)
+| lam_ (_ : v -> term)
 .
 
+Definition lam f := lam_ (fun x => f (var x)).
 End term.
 
 Module TermNotation.
@@ -154,8 +155,8 @@ Notation "_{ e }" := e (e custom lam at level 99).
 Notation "x" := x (in custom lam at level 0, x constr at level 0).
 Notation "f x" := (app f x) (in custom lam at level 1, left associativity).
 Notation "'fun' x => y" :=
-  (lam x y) (in custom lam at level 90,
-                     x constr at level 99,
+  (lam (fun x => y)) (in custom lam at level 90,
+                     x ident,
                      y custom lam at level 99,
                      left associativity).
 Notation "( x )" := x (in custom lam, x at level 99).
@@ -163,191 +164,33 @@ Notation "${ x }" := x (in custom lam, x constr at level 0).
 
 End TermNotation.
 
-Section termf.
-Variables (a b : Set) (f : a -> b).
-
-Fixpoint m (e : @term a) : @term b :=
-match e with
-| var x => var (f x)
-| app e0 e1 => app (m e0) (m e1)
-| lam x e0 => lam (f x) (m e0)
-end.
-
-End termf.
-
-Instance term_Functor : Functor (@term) := { map := m }.
-
-
-(* Find one possible one-hole context of a lambda term on the free variable "x". *)
-
-Section term'.
-
 Import TermNotation.
 
+Section cbn.
 Context {v : Set}.
 
-Definition term' := term (v := v) -> term (v := v).
+Definition store := v -> term (v := v).
 
-Variable x : v.
+Definition st := (store * term (v := v))%type.
 
-Reserved Notation "∈ e" (at level 10).
-Reserved Notation "∉ e" (at level 10).
+CoInductive font : Set := { head : v ; left : font ; right : font }.
 
-Inductive occurs : term -> Prop :=
-| in_var : ∈ (var x)
-| in_lapp {e0 e1} : ∈ e0 -> ∈ _{ e0 e1 }
-| in_rapp {e0 e1} : ∈ e1 -> ∈ _{ e0 e1 }
-| in_lam {y e0} : ∈ e0 -> ∈ _{ fun y => e0 }
-where "∈ e" := (occurs e).
+Definition insert `{EqDec v} x e s : store := fun x' =>
+  if eq_decide x x' then e else s x'.
 
-Inductive not_occurs : term -> Prop :=
-| not_var {y} : x <> y -> ∉ (var y)
-| not_app {e0 e1} : ∉ e0 -> ∉ e1 -> ∉ _{ e0 e1 }
-| not_lam {y e0} : ∉ e0 -> ∉ _{ fun y => e0 }
-where "∉ e" := (not_occurs e).
-
-Inductive D : term -> Set :=
-| var' : D (var x)
-| lapp' {e0 e1} : D e0 -> D _{ e0 e1 }
-| rapp' {e0 e1} : D e1 -> D _{ e0 e1 }
-| lam' {y e0} : D e0 -> D _{ fun y => e0 }
-.
-
-Section atpoint.
-Variable h : term (v := v).
-
-Reserved Notation "∂ y | ∂ x" (at level 0).
-
-Fixpoint diff e (i : D e) :=
-match i with
-| var' => h
-| @lapp' e0 e1 i0 => _{ ${∂e0|∂i0} e1 }
-| @rapp' e0 e1 i1 => _{ e0 ${ ∂e1 | ∂i1 } }
-| @lam' y e0 i0 => _{ fun y => ${ ∂e0|∂i0 } }
-end where "∂ e | ∂ i" := (diff e i).
-
-End atpoint.
-
-Definition var_helper {y} : x = y -> D (var y).
-intro.
-rewrite <- H.
-apply var'.
-Defined.
-
-Fixpoint lookup `{EqDec v} e : D e + { ∉ e } :=
+Fixpoint cbn `{EqDec v} (xs : font) (e : term (v := v)) (s0 : store) :=
 match e with
-| var y =>
-   match eq_decide x y with
-    | left _ eq => inleft (var_helper eq)
-    | right _ neq => inright (not_var neq)
-   end
-| app e0 e1 =>
-   match (lookup e0, lookup e1) with
-   | (inleft e'0, _) => inleft (lapp' e'0)
-   | (_, inleft e'1) => inleft (rapp' e'1)
-   | (inright n0, inright n1) => inright (not_app n0 n1)
-   end
-| lam y e0 =>
-   match lookup e0 with
-     | inleft e'0 => inleft (lam' e'0)
-     | inright n0 => inright (not_lam n0)
-   end
-end .
-
-End term'.
-
-Section variables.
-
-Context { v : Set }.
-
-(* Provide a utility monad *)
-
-(* I think I need to change things to use a partial order not equality *)
-CoInductive stream : Set := { head : v ; tail : stream }.
-
-Definition vars := @state stream.
-Instance vars_Functor : Functor vars := state_Functor.
-Instance vars_Monad : Monad vars vars_Functor := state_Monad.
-
-Import MonadNotation.
-Import TermNotation.
-
-Definition alloc : vars v := do
-  s <- get ; do
-  _ <- put (tail s) ;
-  pure (head s).
-
-
-Definition free (x : v) : vars unit := do
-  s <- get ; do
-  _ <- put {| head := x ; tail := s |} ;
-  pure tt.
-
-
-Section s3.
-Variable x : v.
-Fixpoint replace `{EqDec v} (xs : list (v * v)) :=
-match xs with
-| nil => x
-| cons (y, subst) t => if eq_decide x y is left _ _ then subst else replace t
-end.
-End s3.
-
-Fixpoint rename `{EqDec v} (xs : list (v * v)) (e : term) : vars term :=
-match e with
-| var x => pure (var (replace x xs))
-| _{ f x } => do
-   f' <- rename xs f ; do
-   x' <- rename xs x ;
-   pure _{ f' x' }
-| _{ fun x => e } => do
-   x' <- alloc ; do
-   e' <- rename ((x, x') :: xs) e ;
-   pure _{ fun x' => e' }
+| var x => Some (s0, s0 x)
+| _{ ${lam_ f} e1 } =>
+  let v := head xs in
+  let y := f v in
+  Some (insert v e1 s0, y)
+| _{ e0 e1 } =>
+  if cbn (left xs) e0 s0 is Some (s1, e'0) then Some (s1, _{ e'0 e1 }) else None
+| _ => None
 end.
 
-(* Only recycle bound variables *)
-Fixpoint destroy_term (e : term) : vars unit :=
-match e with
-| var x => pure tt
-| _{ e0 e1 } => do
-  _ <- destroy_term e0 ;
-  destroy_term e1
-| _{ fun x => e0 } => do
-   _ <- destroy_term e0 ;
-   free x
-end
-.
-
-Definition identity: vars term := do
-  x0 <- alloc ; do
-  x1 <- alloc ; 
-  pure _{ (fun x0 => ${var x0}) (fun x1 => ${var x1}) }. 
-
-(*
-Renaming at every substitution should avoid capture AND sharing,
-not sure if that's good or bad.
-Not sure how to double check/formally prove capture is actually avoided.
-*)
-
-Fixpoint step `{EqDec v} e : vars (option term):=
-match e with
-| _{ (fun x => e0) e1 } =>
-  if lookup x e0 is inleft ix then do
-    e'1 <- rename nil e1 ; do
-    e''1 <- rename nil e1 ;
-    pure (Some (let e' := diff x e'1 e0 ix in _{ (fun x => e')  e''1 }))
-  else do
-  _ <- destroy_term e1 ; do
-  _ <- free x ;
-  pure (Some e0)
-| _{ e0 e1 }  => do
-  e'0 <- step e0 ;
-  pure (if e'0 is Some e''0 then Some _{ e''0 e1 } else None)
-| _ => pure None
-end .
-
-End variables.
+End cbn.
 
 Set Primitive Projections.
 
@@ -361,24 +204,67 @@ Extract Inductive option => "Prelude.Maybe" ["Prelude.Just" "Prelude.Nothing"].
 Extract Inductive prod => "(,)" ["(,)"].
 Extract Inductive unit => "()" ["()"].
 Extract Inductive list => "[]" ["[]" "(:)"].
-Extraction "./step.hs" step.
+Extraction "./step.hs" cbn.
 
+Section spec.
 
-(* I think I need to change things to use a partial order not equality *)
-CoInductive font (a : Set) : Set := { head : a ; left : font a ; right : font a }.
+Context {v : Set}.
 
-Definition decide_font v (x y : font v) : {x = y} + {x <> y}.
+(* Define a one-hole context type *)
+Inductive term' : Set :=
+| hole : term'
+| lapp' : term' -> term (v := v) -> term'
+| rapp' : term (v := v) -> term' -> term'
+| lam' : (v -> term') -> term'.
 
+Section substitution.
+Variable h : term (v := v).
+Fixpoint subst i :=
+match i with
+| hole => h
+| lapp' i0 e1 => _{ ${subst i0 } e1 }
+| rapp' e0 i1 => _{ e0 ${ subst i1 } }
+| lam' i0 => lam_ (fun x => subst (i0 x))
+end.
+End substitution.
 
-Instance font_eq {a} : @EqDec (font a).
+Notation "'E' [ h | e ]" := (subst e h) (e custom lam).
+Reserved Notation "e ~> e'" (at level 50).
 
+Inductive reduce : st -> st -> Prop :=
+| reduce_store gamma x : (gamma, var x) ~> (gamma, gamma x)
+| reduce_beta gamma h e0 e1 : (gamma, E[h | (fun x => ${e0 x}) e1 ]) ~> (gamma, E[h | ${e0 e1}])
+where "e ~> e'" := (reduce e e').
 
-Fixpoint approx (fuel : nat) (e : term) : term :=
-if fuel is S n then
-  if step e is Some e' then approx n e' else
-  e else
-e.
+Definition valid f := forall (x : st), if f x is Some y then x ~> y else True.
 
-Eval cbv in (fun v => approx 5 (identity v)).
+Definition strategy := { f | valid f }.
 
-End s1.
+Definition fail : strategy.
+eexists.
+Unshelve.
+2: {
+  intro.
+  apply None.
+}
+easy.
+Defined.
+
+Definition cbn' `{EqDec v} xs x := cbn xs (snd x) (fst x).
+
+Definition cbn_valid `{EqDec v} xs : valid (cbn' xs).
+intro.
+destruct x.
+induction t.
+1: {
+  cbv.
+  apply reduce_store.
+}
+2: {
+  cbv.
+  trivial.
+}
+1: {
+  admit.
+}
+Admitted.
